Add README.md, Add Rerordering.v, fix a bug in Config.t

State.v
@@ -7,41 +7,60 @@ Require Import Value.
 
 Module Ir.
 
+(* Definition of a register file. *)
 Definition regfile := list (nat * Ir.val).
-Definition stack := list (Ir.callid * Ir.IRFunction.pc).
+(* Definition of a call stack. *)
+Definition stack := list (Ir.callid * (Ir.IRFunction.pc * regfile)).
 
 
 Module Config.
 
+(* Definition of a program state. *)
 Structure t := mk
   {
-    r:regfile;
-    m:Ir.Memory.t;
-    s:stack;
+    m:Ir.Memory.t; (* a memory *)
+    s:stack; (* a call stack *)
     cid_to_f:list (Ir.callid * nat); (*callid -> function id*)
-    cid_fresh: Ir.callid;
-    md:Ir.IRModule.t
+    cid_fresh: Ir.callid; (* Fresh, unused call id. *)
+    md:Ir.IRModule.t (* IR module *)
   }.
 
+(* Wellformedness of a program state. *)
 Structure wf (c:t) := mk_wf
   {
+    (* wf_m: Memory is also well-formed. *)
     wf_m: Ir.Memory.wf c.(m);
-    wf_cid_to_f: List.NoDup (List.map fst c.(cid_to_f));
+    (* wf_cid_to_f: there's no duplicated
+       call ids in cid_to_f. which is a mapping from
+       CallID to Function name (= function id)
+       *)
+    wf_cid_to_f: List.NoDup (list_keys c.(cid_to_f));
+    (* wf_cid_to_f2: All function ids in cid_to_f are valid, i.e.,
+       has corresponding function definition. *)
     wf_cid_to_f2: forall cf (HIN:List.In cf c.(cid_to_f)),
         exists f, Ir.IRModule.getf cf.(snd) c.(md) = Some f;
-    wf_stack: forall curcid curpc funid f (HIN:List.In (curcid, curpc) c.(s))
+    (* wf_stack: all PCs stored in the call stack (which is c.(s))
+       are valid, respective to corresponding functions. *)
+    wf_stack: forall curcid curpc funid f curregfile
+                     (HIN:List.In (curcid, (curpc, curregfile)) c.(s))
                      (HIN2:List.In (curcid, funid) c.(cid_to_f))
                      (HF:Some f = Ir.IRModule.getf funid c.(md)),
         Ir.IRFunction.valid_pc curpc f = true
+    (* WIP - more properties will be added later. *)
   }.
 
-
+(* Get register value. *)
 Definition get_rval (c:t) (regid:nat): option Ir.val :=
-  match (List.filter (fun x => Nat.eqb x.(fst) regid) c.(r)) with
+  match c.(s) with
   | nil => None
-  | h::t => Some h.(snd)
+  | (_, (_, r))::_ =>
+    match (List.filter (fun x => Nat.eqb x.(fst) regid) r) with
+    | nil => None
+    | h::t => Some h.(snd)
+    end
   end.
 
+(* Get value of the operand o. *)
 Definition get_val (c:t) (o:Ir.op): option Ir.val:=
   match o with
   | Ir.opconst c => Some
@@ -54,27 +73,36 @@ Definition get_val (c:t) (o:Ir.op): option Ir.val:=
   | Ir.opreg regid => get_rval c regid
   end.
 
+(* Update value of register regid. *)
 Definition update_rval (c:t) (regid:nat) (v:Ir.val): t :=
-  mk ((regid, v)::c.(r)) c.(m) c.(s) c.(cid_to_f) c.(cid_fresh) c.(md).
+  match c.(s) with
+  | nil => c
+  | (cid, (pc0, r))::s' =>
+    mk c.(m) ((cid, (pc0, (regid, v)::r))::s') c.(cid_to_f) c.(cid_fresh) c.(md)
+  end.
 
+(* Update memory. *)
 Definition update_m (c:t) (m:Ir.Memory.t): t :=
-  mk c.(r) m c.(s) c.(cid_to_f) c.(cid_fresh) c.(md).
+  mk m c.(s) c.(cid_to_f) c.(cid_fresh) c.(md).
 
+(* Get function id (= function name) of cid. *)
 Definition get_funid (c:t) (cid:Ir.callid): option nat :=
   match (list_find_key c.(cid_to_f) cid) with
   | nil => None
   | h::t => Some h.(snd)
   end.
 
+(* Update PC into next_pc. *)
 Definition update_pc (c:t) (next_pc:Ir.IRFunction.pc): t :=
   match c.(s) with
-  | (cid, pc0)::t => mk c.(r) c.(m) ((cid,next_pc)::t) c.(cid_to_f) c.(cid_fresh) c.(md)
+  | (cid, (pc0, r))::t => mk c.(m) ((cid,(next_pc, r))::t) c.(cid_to_f) c.(cid_fresh) c.(md)
   | _ => c
   end.
 
+(* Get (definition of the running function, PC inside the function). *)
 Definition cur_fdef_pc (c:t): option (Ir.IRFunction.t * Ir.IRFunction.pc) :=
   match (Ir.Config.s c) with
-  | (cid, pc0)::t =>
+  | (cid, (pc0, _))::t =>
     match Ir.Config.get_funid c cid with
     | Some funid =>
       match Ir.IRModule.getf funid c.(md) with
@@ -86,6 +114,7 @@ Definition cur_fdef_pc (c:t): option (Ir.IRFunction.t * Ir.IRFunction.pc) :=
   | nil => None
   end.
 
+(* Returns true if the call stack has more than one entry, false otherwise. *)
 Definition has_nestedcall (c:t): bool :=
   Nat.ltb 1 (List.length (Ir.Config.s c)).
 
