README.md
@@ -1,0 +1,47 @@
+### About
+
+This is a Coq formalization of OOPSLA'18 LLVM memory model.
+
+
+### Definition of Memory
+
+- Definition of memory: `Ir.Memory.t` in [Memory.v](Memory.v)
+    + `Ir.Memory.t` means `t` in `Mdoule Memory` in `Module Ir`.
+
+- Well-formedness of a memory: `Ir.Memory.wf` in [Memory.v](Memory.v)
+
+- Definition of a memory block: `Ir.MemBlock.t` in [Memory.v](Memory.v)
+
+- Well-formedness of a memory block: `Ir.MemBlock.wf` in [Memory.v](Memory.v)
+
+- Definition of dereferenceability: `Ir.deref` in [LoadStore.v](LoadStore.v)
+
+- Semantics of load/store: `Ir.load_val`/`Ir.store_val` in [LoadStore.v](LoadStore.v)
+
+
+### Definition of IR syntax & Program Behavior
+
+- Definition of IR syntax: [Lang.v](Lang.v)
+    + Phi node: `Ir.PhiNode.t` (or 't' in `Module PhiNode` in `Module Ir`)
+    + Instruction: `Ir.Inst.t`
+    + Terminator: `Ir.Terminator.t`
+    + Basic block: `Ir.BasicBlock.t`
+    + Function: `Ir.IRFunction.t`
+    + Module: `Ir.IRModule.t`
+
+- Definition of small-step semantics of IR instructions: [SmallStep.v](SmallStep.v)
+
+- Definition of a program state: `Ir.Config.t` in [State.v](State.v)
+
+- Well-formedness of a program state: `Ir.Config.wf` in [State.v](State.v)
+
+- Definition of an event: `event` in [Behaviors.v](Behaviors.v)
+
+- Definition of a program behavior: `Ir.program_behavior` in [Behaviors.v](Behaviors.v)
+
+- Definition of refinement : `Ir.refines` in [Behaviors.v](Behaviors.v)
+
+
+### Proofs
+
+- Reordering of interested instructions: [Reordering.v](Reordering.v) 
